\documentclass[12pt]{article}
\parindent0pt
\usepackage{ctex}
\usepackage{amsmath}
\usepackage{mathtools,amssymb}
\title{assignemnt 5}
\author{Longyu Zhu}

\begin{document}

\section*{2.4}
\subsection*{Exercise 12}
a)$a_{n}=0$\\
replace n in $a_n=0$ by n-1 and n-2:\\
$a_{n-1}=0$\\
$a_{n-2}=0$\\
$-3a_{n-1}+4a_{n-2}=-3(0)+4(0)=0+0=a_n$\\

b)$a_{n}=1$\\
same with a just change $a_{n}=1$\\
we will get$-3a_{n-1}+4a_{n-2}=-3(1)+4(1)=-3+4=1=a_n$\\

c)$a_{n}=(-4)^n$\\
\begin{equation}\nonumber
    \begin{split}
        -3a_{n-1}+4a_{n-2} & =-3(-4)^{n-1}+4(-4)^{n-2}\\
          & =3*(-4)*(-4)^{n-2}+4(-4)^{n-2}\\
          & =(-4)^{n-2}(-3*(-4)+4)\\
          & =(-4)^{n-2}(12+4)\\
          & =(-4)^{n-2}(16)\\
          & =(-4)^{n-2}(-4)^{-2}\\
          & =(-4)^n\\
          & =a_{n}
    \end{split}
\end{equation}

d)$a_{n}=2(-4)^n+3$\\
\begin{equation}\nonumber
    \begin{split}
        -3a_{n-1}+4a_{n-2} &=-3(2(-4)^{n-1}+3)+4(2(-4)^{n-2}+3)\\
        &=-6(-4)^{n-1}-9+8(-4)^{n-2}+12\\
        &=(-6(-4)^{n-1}+8(-4)^{n-2}+12)\\
        &=(-6*(-4)*(-4)^{n-2}+8(-4)^{n-2})+3\\
        &=(-4)^{n-2}(-6*(-4)+8)+3\\
        &=(-4)^{n-2}(24+8)+3\\
        &=(-4)^{n-2}*32+3\\
        &=(-4)^{n-2}*16*2+3\\
        &=(-4)^{n-2}*(-4)^2*2+3\\
        &=(-4)^{n}*2+3\\
        &=2(-4)^n+3\\
        &=a_n
    \end{split}
\end{equation}


\subsection*{Exercise 16}
a)$a_{n}=-a_{n-1},a_0=5$\\
\begin{equation}\nonumber
    \begin{split}
        a_n&=-a_{n-1}=(-1)^1*a_{n-1}\\
        &=-a_{n-2}=(-1)^2*a_{n-2}\\
        &=-a_{n-3}=(-1)^3*a_{n-3}\\
        &=-a_{n-4}=(-1)^4*a_{n-4}\\
        &=(-1)^na_{n-n}\\
        &=(-1)^na_0\\
        &=5(-1)^n
    \end{split}
\end{equation}

b)$a_{n}=a_{n-1}+3,a_0=1$\\
\begin{equation}\nonumber
    \begin{split}
        a_n&=a_{n-1}+3=a_{n-1}+3*1\\
        &=a_{n-2}+3*1=a_{n-1}+6=a_{n-2}+3*2\\
        &=a_{n-3}+3*2=a_{n-1}+9=a_{n-2}+3*3\\
        &=a_{n-4}+3*3=a_{n-1}+12=a_{n-2}+3*4\\
        &=a_{n-n}+3*n\\
        &=a_0+3n\\
        &=1+3n\\
        &3n+1
    \end{split}
\end{equation}

c)$a_{n}=a_{n-1}-n,a_0=4$\\
\begin{equation}\nonumber
    \begin{split}
        a_n&=a_{n-1}-n=a_{n-1}-n+0\\
        &=(a_{n-2}-(n-1))-n=a_{n-2}-2n+0+1\\
        &=(a_{n-3}-(n-2))-2n+1=a_{n-3}-3n+0+1+2\\
        &=(a_{n-4}-(n-3))-3n+3=a_{n-4}-4n+0+1+2+3\\
        &=a_0-n^2+\frac{n-1}{n}\\
        &=4-n^2+\frac{n^2-n}{2}\\
        &=-\frac{1}{2}n^2-\frac{1}{2}n+4
    \end{split}
\end{equation}

d)$a_{n}=2a_{n-1}-3,a_0=-1$\\
\begin{equation}\nonumber
    \begin{split}
        a_n&=2a_{n-1}-3=2^1a_{n-1}-3\\
        &=2(2a_{n-2}-3)-3=2^2a_{n-2}-(3*2^0+3*2^1)\\
        &=2^2(2a_{n-3}-3)-(3*2^0+3*2^1)=2^3a_{n-2}-(3*2^0+3*2^1+3*2^2)\\
        &=2^3(2a_{n-3}-3)-(3*2^0+3*2^1+3*2^2)=2^4a_{n-2}-(3*2^0+3*2^1+3*2^2+3*2^3)\\
        &=2^n*(-1)-3*\frac{2^n-1}{2-1}\\
        &=-2^n-3(2^n-1)\\
        &=-2^n-3*2^n+3\\
        &=-4*2^n+3
    \end{split}
\end{equation}

e)$a_{n}=(n+1)a_{n-1},a_0=2$\\
\begin{equation}\nonumber
    \begin{split}
        a_n&=(n+1)a_{n-1}\\
        &=(n+1)(n)a_{n-2}\\
        &=(n+1)(n)(n-1)a_{n-3}\\
        &=(n+1)(n)(n-1)(n-2)a_{n-4}\\
        &=(n+1)!a_0\\
        &=(n+1)!*2\\
        &=2*(n+1)!
    \end{split}
\end{equation}


f)$a_{n}=2na_{n-1},a_0=3$\\
\begin{equation}\nonumber
    \begin{split}
        a_n&=2na_{n-1}=2^1na_{n-1}\\
        &=2n(2(n-1)a_{n-2})=2^2n(n-1)a_{n-2}\\
        &=2^2n(n-1)(2(n-2)a_{n-2})=2^3n(n-1)(n-2)a_{n-3}\\
        &=2^3n(n-1)(n-2)(2(n-3)a_{n-2})=2^4n(n-1)(n-2)(n-3)a_{n-4}\\
        &=2^n*n!*a_0\\
        &=2^n*n!*3\\
        &=3n!2^n
    \end{split}
\end{equation}

g)$a_{n}=-a_{n-1}+n-1,a_0=7$\\
\begin{equation}\nonumber
    \begin{split}
        a_n=-a_{n-1}+n-1&=(-1)^1a_{n-1}+(n-1)\\
        &=(-1)^2a_{n-2}+((n-1)-(n-2))\\
        &=(-1)^3a_{n-3}+((n-1)-(n-2)+(n+3))\\
        &=(-1)^4a_{n-4}+((n-1)-(n-2)+(n+3)-(n-4))\\
        &=(-1)^na_0+\sum_{i=0}^{n-1}(-1)^{n-i+1}i\\
        &=7*(-1)^n+\sum_{i=0}^{n-1}(-1)^{n-i+1}i\\
    \end{split}
\end{equation}

\section*{2.5}
\subsection*{Exercise 2}
a) the integers greater than 10 \\
f(n)=n+10, Countably infinite\\

b) the odd negitive integers.\\
f(n)=1-2n, Countably infinite\\

c)the integers with absolute value less than 1,000,000 .\\
$C=\{x:\|x\|<1,000,000\}\\
C=\{x:-1,000,000<x<1,000,000\}$\\
Finite\\

d) the real number between 0 and 2. \\
$D=\{x:x\in (0,2)\cap R\}$\\
uncountable\\

e) the set A*$Z^+$ where $A=\{2,3\}$.\\
Countably infinite\\
by f(2,n)=2n and f(3,n)\\

f) the intergers are multiples of 10. \\
Countably infinite\\
$F=\{10n:n\in Z\}$\\
Countably infinite\\


\subsection*{Exercise 10}
a) finite.\\
A=all real number =0\\
B=all real number >0\\
$A-B=\varnothing $\\

b) countably infinite.\\
A=all real number\\
B=all real number that are not the positive intergers\\
 $=A-()^+$\\
A-B=A-$(A-()^+)$\\
=$()^+$\\

c) uncountable.\\
A=all real number\\
B=all positive real number\\
A-B=$\{0,R^-\}$\\

\end{document} 